coq/theories/ITree/Delay.v
@@ -14,3 +14,16 @@ Definition emb_delay {I} {E : event I I} {X i} : delay X -> itree E (X @ i) i :=
          | TauF t => TauF (_emb_delay t)
          | VisF e k => match e with end
          end).
+
+Definition subst_delay {I} {E : event I I} {X Y i} (f : X -> itree E Y i)
+           : delay X -> itree E Y i :=
+  cofix _subst_delay x :=
+    go (match x.(_observe) with
+       | RetF r => (f r).(_observe)
+       | TauF t => TauF (_subst_delay t)
+       | VisF e k => match e with end
+       end).  
+
+Definition bind_delay {I} {E : event I I} {X Y i}
+  : delay X -> (X -> itree E Y i) -> itree E Y i
+  := fun x f => subst_delay f x .
